various advances, eg flatten in utilities is now shorter and linear. Last commit before trying to look over and unify how the types of the constructors of an inductive are computed

interpretation_algebraic_types.v
@@ -60,10 +60,10 @@ MetaCoq Quote Definition or_reif := Eval cbn in or.
 
 (** reified equalities **)
 
-Definition mkNamed s := ({| binder_name := nNamed (s%string); binder_relevance := Relevant |} : aname).
+(* Definition mkNamed s := ({| binder_name := nNamed (s%string); binder_relevance := Relevant |} : aname).
 Definition mkNAnon := {| binder_name := nAnon; binder_relevance := Relevant |}.
 
-Definition mkNamedtry := mkNamed (("B"%string) : ident).
+Definition mkNamedtry := mkNamed (("B"%string) : ident).*)
 
 
 Definition consS_typ := tProd (mkNamed "A") (tSort (Universe.from_kernel_repr (Level.lSet, false) []))
@@ -107,18 +107,6 @@ Fixpoint or_nary_reif (l : list term):=
   end.
 
 
-Definition dom_list_f ( B  :  term) (n : nat)  := (* \TODO transfer in utilities.v *)
-  (* takes a type B := Prod A1 ... An . B'  and outputs (B,[A1; ... ; An]), at least if no dependencies *)
-  (* does not handle debruijn indices *)
-  let fix dlaux B n acc :=
-  match n with
-  | 0 => (B,tr_rev acc) 
-  | S n => match B with
-          | tProd na A B' =>  dlaux B' n (A :: acc)
-          | _ => (B,[]) (* this case shouldn't happen *)
-          end            
-  end
-  in dlaux B n [].
 
 
 
@@ -490,13 +478,17 @@ Ltac inj_disj_tac lB lf lA ln p  :=
   lazymatch eval hnf in lB with
    | ?B :: ?tlB => ctors_are_inj_tac lB lf lA ln p ; pairw_disj_codom_tac B lf lA  p
     end.
+
 Definition list_ctor_oind ( oind : one_inductive_body ) : list term :=
   let fix list_lctor ( l : list ((ident × term) × nat )) acc :=
   match l with
-  | [] => []
+  | [] => acc
   | ((idc , ty) , n ) :: tlctor => list_lctor  tlctor  (ty :: acc) 
   end in  tr_rev (list_lctor oind.(ind_ctors) []).
   
+
+
+
 Definition switch_inductive ( indu : inductive) (i : nat) :=
   match indu with 
   | {| inductive_mind := kn ; inductive_ind := k |} => {| inductive_mind := kn ; inductive_ind := i |}
